src/impl/TLS13.Impl.Handle.Local.fst
@@ -7,9 +7,11 @@ open Pulse.Lib.Array.PtsTo
 open TLS13.Impl.Client.Types
 
 module B = TLS13.Bytes
+module CL = TLS13.ConnectionLog
 module C = TLS13.Impl.ConnectionState
 module CS = TLS13.Spec.ConnectionState
 module CT = TLS13.Impl.Client.Types
+module M = TLS13.Messages
 module Seq = FStar.Seq
 module SZ = FStar.SizeT
 module U8 = FStar.UInt8
@@ -36,18 +38,18 @@ fn handle_local_event
                    kind
                    (Ghost.reveal 'payload_bytes))
   returns resp: CT.client_response
-  ensures exists* st1.
+  ensures exists* st1 network_out_bytes.
           C.connection_exactly c st1 **
           pts_to payload 'payload_bytes **
-          pts_to network_out 'old_network_out **
+          pts_to network_out network_out_bytes **
           pts_to app_out 'old_app_out **
-          pure (B.length 'old_network_out == SZ.v network_out_len /\
+          pure (B.length network_out_bytes == SZ.v network_out_len /\
                 B.length 'old_app_out == SZ.v app_out_len /\
                 CT.some_legal_response
                   'st0
                   st1
                   resp
-                  'old_network_out
+                  network_out_bytes
                   'old_app_out /\
                 CT.legal_handled_local_response
                   'st0
@@ -55,7 +57,7 @@ fn handle_local_event
                   resp
                   kind
                   (Ghost.reveal 'payload_bytes)
-                  'old_network_out
+                  network_out_bytes
                   'old_app_out)
 {
   match kind {
@@ -868,6 +870,101 @@ fn handle_local_event
         (C.local_fail_state 'st0 C.tls_unexpected_message_error)
         resp
         CT.LocalVerifyFinished
+        (Ghost.reveal 'payload_bytes)
+        'old_network_out
+        'old_app_out));
+      assert (pure (CT.some_legal_response
+        'st0
+        (C.local_fail_state 'st0 C.tls_unexpected_message_error)
+        resp
+        'old_network_out
+        'old_app_out));
+      resp
+    }
+  }
+    LocalSendClientFinished -> {
+    let ok = C.try_send_client_finished c network_out network_out_len;
+    if ok {
+      with fin raw_sent network_out_bytes.
+        assert (pts_to network_out network_out_bytes);
+      assert (C.connection_exactly c (C.sent_client_finished_state 'st0 fin raw_sent));
+      assert (pure (B.length network_out_bytes == SZ.v network_out_len));
+      assert (pure (58 <= B.length network_out_bytes));
+      assert (pure (C.can_send_client_finished 'st0 fin raw_sent));
+      assert (pure (Seq.equal raw_sent (Seq.slice network_out_bytes 0 58)));
+      let resp = {
+        CT.network_out_len = 58sz;
+        CT.app_out_len = 0sz;
+        CT.status = CT.StepOk;
+      };
+      assert (pure (58 <= B.length network_out_bytes));
+      Seq.lemma_len_slice network_out_bytes 0 58;
+      assert (pure (Seq.equal raw_sent (CT.response_network_out resp network_out_bytes)));
+      Seq.lemma_len_slice 'old_app_out 0 0;
+      Seq.lemma_eq_intro B.empty (Seq.slice 'old_app_out 0 0);
+      C.lemma_sent_client_finished_state_evolves 'st0 fin raw_sent;
+      assert (pure (CT.legal_response_for_event
+        'st0
+        (C.sent_client_finished_state 'st0 fin raw_sent)
+        resp
+        (CS.ConnNetworkEvent {
+          CL.message_direction = CL.Sent;
+          CL.message_value = M.TlsHandshake (M.Finished fin);
+        })
+        raw_sent
+        B.empty
+        network_out_bytes
+        'old_app_out));
+      assert (pure (CT.legal_local_response
+        'st0
+        (C.sent_client_finished_state 'st0 fin raw_sent)
+        resp
+        CT.LocalSendClientFinished
+        (Ghost.reveal 'payload_bytes)
+        (CS.ConnNetworkEvent {
+          CL.message_direction = CL.Sent;
+          CL.message_value = M.TlsHandshake (M.Finished fin);
+        })
+        raw_sent
+        B.empty
+        network_out_bytes
+        'old_app_out));
+      assert (pure (CT.legal_handled_local_response
+        'st0
+        (C.sent_client_finished_state 'st0 fin raw_sent)
+        resp
+        CT.LocalSendClientFinished
+        (Ghost.reveal 'payload_bytes)
+        network_out_bytes
+        'old_app_out));
+      assert (pure (CT.some_legal_response
+        'st0
+        (C.sent_client_finished_state 'st0 fin raw_sent)
+        resp
+        network_out_bytes
+        'old_app_out));
+      resp
+    } else {
+      C.mark_unexpected_message c;
+      let resp = {
+        CT.network_out_len = 0sz;
+        CT.app_out_len = 0sz;
+        CT.status = CT.IllegalTransition;
+      };
+      Seq.lemma_len_slice 'old_network_out 0 0;
+      Seq.lemma_eq_intro B.empty (Seq.slice 'old_network_out 0 0);
+      assert (pure (Seq.equal B.empty (CT.response_network_out resp 'old_network_out)));
+      assert (pure (CT.unexpected_message_response
+        'st0
+        (C.local_fail_state 'st0 C.tls_unexpected_message_error)
+        resp
+        'old_network_out
+        'old_app_out));
+      assert (pure (CT.legal_handled_local_response
+        'st0
+        (C.local_fail_state 'st0 C.tls_unexpected_message_error)
+        resp
+        CT.LocalSendClientFinished
         (Ghost.reveal 'payload_bytes)
         'old_network_out
         'old_app_out));
